examples/unit-tests/encrypt.fst
@@ -1,0 +1,122 @@
+
+module AES (* concrete implementation of a one-block symmetric cipher *)
+open Array
+
+type bytes = seq byte
+type nbytes (n:nat) = b:bytes{length b == n}
+
+let blocksize = 32 (* 256 bits *)
+
+type plain  = nbytes blocksize
+type cipher = nbytes (2 * blocksize)  (* including IV *)
+
+let keysize = 16 (* 128 bits *)
+type key = nbytes keysize 
+
+assume val generated : key -> Tot bool
+
+assume val gen: unit -> key 
+assume val dec: key -> cipher -> Tot plain                    (* this function is pure & complete *)  
+assume val enc: k:key -> p:plain -> c:cipher { dec k c = p }  (* this function is not pure (IV); the refinement captures functional correctness *) 
+
+
+module SymEnc (* a multi-key symmetric variant; for simplicity: (1) only using AES above; and (2) parsing is complete *)
+
+(* TODO: we get the index from a counter; 
+   In the crypto argument, we rely on the fact that we only construct keys once for each i. *)
+
+assume type keyval (p:Type) (r:Type) (i:int)
+
+(* TODO ???
+opaque type keyval (p:Type) (r:Type) (i:int) = 
+  | Ideal    : (plain: r -> p) -> (repr: p -> r) -> AES.key -> keyval p r i   (* maybe no need to keep plain/repr around *)
+  | Concrete : (plain: r -> p) -> (repr: p -> r) -> AES.key -> keyval p r i 
+ *)
+
+type key (p:Type) (r:Type) = i:int * keyval p r i (* so that the index i can be kept implicit *)
+
+(* CPA variant: *) 
+
+logic type Encrypted: #p: Type -> #r: Type -> key p r -> AES.cipher -> Type (* an opaque predicate, keeping track of honest encryptions *)
+
+type cipher (p:Type) (r:Type) (k: key p r) = c: AES.cipher { Encrypted #p #r k c }    (* TODO why do I need explicit implicits? *)
+
+assume val keygen:  #p:Type -> #r:Type -> (plain: r -> p) -> (repr: p -> r) -> key p r 
+assume val decrypt: #p:Type -> #r:Type -> k:key p r -> cipher p r k -> Tot p
+assume val encrypt: #p:Type -> #r:Type -> k:key p r -> plain: p -> c:cipher p r k { decrypt k c = plain }
+
+(*
+
+(* TODO: implementation *)
+
+//let c = ref 0
+
+let keygen safe plain repr = 
+//let i = !c in
+//c := !c + 1; 
+  let i = 3 in
+  let k = AES.gen() in 
+  if safe 
+  then i, Ideal   (plain,repr,k) 
+  else i, Concrete(plain,repr,k)
+
+let decrypt (i,Ideal(plain,repr,kv)) c = AES.dec kv c
+let encrypt (i,Ideal(plain,repr,kv)) p = AES.enc kv p
+
+
+(* below is for CCA2, with just bytes as ciphers. *)
+
+assume val decrypt: p:Type -> r:Type -> k:key p r -> c: cipher -> option p 
+assume val encrypt: p:Type -> r:Type -> k:key p r -> plain: p -> c:cipher { decrypt p r k c = Some plain }
+
+(* for CPA, ciphers should not be forgeable, but we need to be able to treat sbytes as cipher after checking e.g. a MAC *)
+
+assume val decrypt: p:Type -> r:Type -> k:skey p r -> c: cipher p r k -> option p 
+assume val encrypt: p:Type -> r:Type -> k:skey p r -> plain: p -> c:cipher p r k { decrypt p r k c = plain }
+*)
+
+module SampleEncrypt
+
+let plain (x:AES.plain) = x 
+let repr (x:AES.plain) = x 
+
+let test() = 
+  let p = failwith "nice bytes" in
+  let k0 = SymEnc.keygen plain repr in
+  let k1 = SymEnc.keygen plain repr in
+  let c = SymEnc.encrypt k0 p in
+  let p' = SymEnc.decrypt k0 c in 
+  assert( p == p');                   // this succeeds, by functional correctness
+//  let p'' = SymEnc.decrypt k1 c in  // this rightfully triggers an error
+  ()
+
+
+module EncryptThenMAC 
+
+type key (p:Type) (r:Type) = 
+  | Key:  ke:SymEnc.key p r -> MacIdeal.pkey (fun c -> SymEnc.Encrypted ke c) -> key p r 
+
+type cipher = AES.cipher * MacIdeal.tag
+
+val keygen:  #p:Type -> #r:Type -> (plain: r -> p) -> (repr: p -> r) -> key p r 
+assume val decrypt: #p:Type -> #r:Type -> k:key p r -> cipher -> Tot (option p)
+val encrypt: #p:Type -> #r:Type -> k:key p r -> plain: p -> c:cipher { decrypt #p #r k c = Some plain }
+
+let keygen plain repr = 
+  let ke = SymEnc.keygen plain repr in
+  let ka = MacIdeal.new_key (fun c -> SymEnc.Encrypted ke c) in 
+  Key ke ka
+
+(*
+let encrypt (ke,ka) plain = 
+  let c = SymEnc.encrypt ke plain in
+  (c, MacIdeal.mac ka c)
+
+let decrypt (ke,ka) plain = 
+  let c = SymEnc.encrypt ke plain in
+  (c, MacIdeal.mac ka c)
+
+
+
+
+ *)
